added state law and theorem

PSBP/Laws/WithStateLaws.lean
@@ -4,27 +4,22 @@ import PSBP.Specifications.WithStateSpecification
 
 import PSBP.Structures.ComputationValuedFunction
 
-class LawfulStateOf (computation : Type → Type)
+class LawfulStateOf (σ : Type) (computation : Type → Type)
     [Monad computation]
     [MonadStateOf σ computation] : Prop where
   stateOf_write_read :
-    (λ σ => set σ >>= λ _ : PUnit => get) =
-      (pure : σ → computation σ)
+    ((λ s => set s >>= λ _ => getThe σ) : σ → computation σ) =
+      (pure)
 
-@[simp] theorem stateOf_write_read_theorem
-  {σ : Type}
-    [Monad computation]
-    [MonadStateOf σ computation] :
-  (λ σ => set σ >>= λ _ : PUnit => get
-    : σ → computation σ ) =
-      (pure : σ → computation σ) :=
-        sorry
+export LawfulStateOf (stateOf_write_read)
 
-class LawfulWithState (program : Type → Type → Type)
+attribute [simp] stateOf_write_read
+
+class LawfulWithState
     [Functional program]
     [Sequential program]
     [WithState σ program] : Prop where
   withState_write_read :
-    (writeState >=> (readState : program Unit σ)) =
+    ((writeState : program σ Unit) >=>
+      (readState : program Unit σ)) =
       identity
-
