PSBP/Evaluations/Programs.lean
@@ -7,7 +7,7 @@ import PSBP.Materializations.TaskMaterialization
 import PSBP.Programs.Programs
 
 #eval
-  materializeActive fibonacci 10 ==
+  materializeActive fibonacci 24 ==
     89
 
 #eval
