PSBP/Implementations/WithStateImplementation.lean
@@ -7,5 +7,5 @@ import PSBP.Structures.ComputationValuedFunction
 instance [MonadStateOf σ computation] :
     WithState σ
       (FromComputationValuedFunction computation) where
-  readState := ⟨λ _ => get⟩
+  readState := ⟨λ _ => getThe σ⟩
   writeState := ⟨set⟩
