PSBP/Materializations/TaskMaterialization.lean
@@ -2,10 +2,16 @@ import PSBP.Structures.ComputationValuedFunction
 
 import PSBP.Implementations.ProgramImplementations
 
+instance : Monad Task where
+  pure := Task.pure
+  bind := Task.bind
+
+instance : MonadAsync Task where
+  async := Task.spawn
+
 abbrev TaskProgram :=
   FromComputationValuedFunction Task
 
 def materializeTask {α β : Type} :
   TaskProgram α β → (α → β) :=
     λ ⟨αftβ⟩ α => (αftβ α).get
-
