PSBP/Theorems/WithStateTheorems.lean
@@ -1,3 +1,17 @@
-def foo : Nat := 1
+import PSBP.Specifications.ProgramSpecifications
 
+import PSBP.Structures.ComputationValuedFunction
 
+import PSBP.Implementations.ProgramImplementations
+
+import PSBP.Implementations.WithStateImplementation
+
+import PSBP.Laws.WithStateLaws
+
+@[simp] theorem withState_write_read
+    [Monad computation]
+    [MonadStateOf σ computation]
+    [LawfulStateOf σ computation] :
+  ((writeState >=> readState) :
+      FromComputationValuedFunction computation σ σ) =
+    identity := by simp [andThenP, identity, asProgram]
